checkpoint

Veritas.Verifier.TSLog.fst
@@ -828,6 +828,24 @@ let lemma_eac_value_correct_type (itsl: eac_log) (k:key)
     lemma_reduce_empty EACInit (trans_fn (seq_machine_of eac_sm));
     aux 0 EACInit
 
+let eacs_t (itsl:eac_log) = k:key -> e:eac_state { e == eac_state_of_key itsl k /\ e <> EACFail }
+let threads_t (itsl:eac_log) = t:valid_tid itsl -> v:vtls { Valid? v /\ v == verify (t, Seq.index (I.s_seq itsl) t) }
+noeq 
+type monitored_state (itsl:eac_log) = {
+  eacs: eacs_t itsl;
+  threads: threads_t itsl
+}
+
+let eq_mon itsl (m0 m1: monitored_state itsl) = 
+  FunctionalExtensionality.feq m0.eacs m1.eacs /\
+  FunctionalExtensionality.feq m0.threads m1.threads
+  
+let run_monitor (itsl:eac_log) 
+  : monitored_state itsl 
+  = let eacs : eacs_t itsl = fun k -> eac_state_of_key itsl k in
+    let threads : threads_t itsl = fun t -> verify (thread_log (I.s_seq itsl) t) in
+    { eacs; threads }
+  
 
 #push-options "--ifuel 0,0 --fuel 1,1"
 (* we never see operations on Root so its eac state is always init *)
@@ -896,11 +914,152 @@ let lemma_eac_state_init_store (itsl: eac_log) (k: key) (tid:valid_tid itsl)
     assert (SA.prefix thread_log_tid 0 `Seq.equal` empty);
     aux 0 (init_thread_state tid)
 
+let t_verify_step_framing (v:vtls{Valid? v}) (e:vlog_entry) (k:key{key_of e <> k})
+  : Lemma (let open Veritas.Verifier in
+           let v' = t_verify_step v e in
+           Valid? v' ==>
+           thread_store v' k == thread_store v k)
+  = admit()           
+
+
+#push-options "--ifuel 1,1 --fuel 1,1 --z3rlimit_factor 4"
 (* when the eac state of a key is evicted then no thread contains the key in its store *)
-let lemma_eac_state_evicted_store  (itsl: eac_log) (k: key{is_eac_state_evicted itsl k}) 
-  (tid:valid_tid itsl):
-  Lemma (not (store_contains (thread_store itsl tid) k))
- = admit()
+let lemma_eac_state_evicted_store (itsl: eac_log) 
+                                  (k: key{is_eac_state_evicted itsl k}) 
+                                  (tid:valid_tid itsl)
+ : Lemma (not (store_contains (thread_store itsl tid) k))
+ = let evicted eacs = (EACEvictedBlum? eacs || EACEvictedMerkle? eacs) in
+   let filter_fn = iskey #(key_type eac_sm) (partn_fn eac_sm) k in 
+   let rec aux (itsl:eac_log)
+               (m:monitored_state itsl)
+     : Lemma (ensures 
+                forall (tid:valid_tid itsl). 
+                  evicted (m.eacs k) ==>
+                  not (store_contains (Valid?.st (m.threads tid)) k))
+             (decreases (I.length itsl))
+     = if I.length itsl = 0
+       then (
+         let vl = vlog_ext_of_its_log itsl in
+         assert (vl `Seq.equal` empty);
+         let vl' = partn eac_sm k vl in
+         lemma_filter_empty filter_fn;
+         assert (vl' `Seq.equal` empty);
+         lemma_reduce_empty EACInit (trans_fn (seq_machine_of eac_sm));
+         assert (m.eacs k == EACInit)
+       )
+       else (
+         let itsl' = I.prefix itsl (I.length itsl - 1) in
+         let m' = run_monitor itsl' in
+         aux itsl' m'; 
+         assert (forall (tid:valid_tid itsl).
+                   evicted (m'.eacs k) ==>
+                   not (store_contains (Valid?.st (m'.threads tid)) k));
+         let i = I.length itsl - 1 in
+         let v = I.index itsl i in
+         let ve = mk_vlog_entry_ext itsl i in
+         let vl' = vlog_ext_of_its_log itsl' in
+         let vl'_k = partn eac_sm k vl' in
+         let vl = vlog_ext_of_its_log itsl in
+         let vl_k = partn eac_sm k vl in
+         assume (vl `Seq.equal` Seq.snoc vl' ve);
+         if filter_fn ve
+         then admit()
+         else (
+           assume (vl'_k `Seq.equal` vl_k);
+           assert (m.eacs k == m'.eacs k);
+           let tid = thread_id_of itsl i in
+           let rec aux (tid':valid_tid itsl)
+             : Lemma 
+               (requires evicted (m.eacs k))
+               (ensures not (store_contains (Valid?.st (m.threads tid')) k))
+               [SMTPat (m.threads tid')]
+             = if tid' = tid
+               then (
+                 let _, tl' = thread_log (I.s_seq (I.prefix itsl i)) tid' in
+                 let _, tl = thread_log (I.s_seq itsl) tid' in
+                 assume (tl `Seq.equal` Seq.snoc tl' v);
+                 assert (SA.prefix tl (Seq.length tl - 1) `Seq.equal` tl');
+                 assert (m'.threads tid' == verify (tid', tl'));
+                 assert (m.threads tid' == t_verify_step (m'.threads tid') v);
+                 let st' = Valid?.st (m'.threads tid') in
+                 let st =  Valid?.st (m.threads tid') in
+                 assert (evicted (m'.eacs k));
+                 assert (not (store_contains (Valid?.st (m'.threads tid')) k));
+                 assert (key_of v <> k);
+                 t_verify_step_framing (m'.threads tid') v k;
+                 assert (st k == st' k)
+               )
+               else (
+                  assume (thread_log (I.s_seq itsl) tid' ==
+                          thread_log (I.s_seq (I.prefix itsl i)) tid');
+                  assert (m.threads tid' == m'.threads tid')
+               )
+           in
+           ()
+         )
+       )
+   in
+   let m = run_monitor itsl in
+   aux itsl m;
+   assert (evicted (m.eacs k));
+   assert (thread_store itsl tid == Valid?.st (m.threads tid))
+
+ 
+ 
+ let _, thread_log_tid = thread_log (s_seq itsl) tid in
+   let thread_state_tid = verify (tid, thread_log_tid) in
+   let store_tid = Valid?.st thread_state_tid in
+   let vl = vlog_ext_of_its_log itsl in
+   let eacs = eac_state_of_key itsl k in
+
+   assert (evicted eacs);
+   let filter_fn = iskey #(key_type eac_sm) (partn_fn eac_sm) k in
+   let vl' : seq vlog_entry_ext = partn eac_sm k vl in
+   assert (eacs == seq_machine_run (seq_machine_of eac_sm) vl');
+   lemma_eac_state_of_root_init itsl;
+   assert (k <> Root); //state of Root should be init
+   let rec aux (j:nat{j <= Seq.length vl'})
+               (eacs:eac_state{eacs == seq_machine_run (seq_machine_of eac_sm) (SA.prefix vl' j)})
+     : Lemma (requires 
+               forall
+               (ts:vtls{ ts == verify (tid, SA.prefix thread_log_tid i) /\
+                        (Valid? ts /\ evicted eacs ==> not (store_contains (Valid?.st ts) k)) })
+   
+
+   let rec aux (i:nat{i <= Seq.length thread_log_tid})
+               (j:nat{j <= Seq.length vl' /\ (j = Seq.length vl' ==> i = Seq.length thread_log_tid)})
+               (eacs:eac_state{eacs == seq_machine_run (seq_machine_of eac_sm) (SA.prefix vl' j)})
+               (ts:vtls{ ts == verify (tid, SA.prefix thread_log_tid i) /\
+                        (Valid? ts /\ evicted eacs ==> not (store_contains (Valid?.st ts) k)) })
+      : Lemma (ensures not (store_contains store_tid k))
+              (decreases (Seq.length vl' - j))
+      = if j = Seq.length vl'
+        then (
+          assert (SA.prefix vl' j `Seq.equal` vl');
+          assert (SA.prefix thread_log_tid i `Seq.equal` thread_log_tid)
+        )
+        else (
+          let ve = Seq.index vl' j in
+          let eacs' = eac_add ve eacs in
+          assert (SA.prefix vl' (j + 1) `Seq.equal` (Seq.snoc (SA.prefix vl' j) ve));
+          lemma_reduce_append EACInit (trans_fn (seq_machine_of eac_sm)) (SA.prefix vl' j) ve;
+          assert (seq_machine_run (seq_machine_of eac_sm) (SA.prefix vl' (j + 1)) ==
+                  eacs');
+          let j' = filter_index_map filter_fn vl j in
+          assert (Seq.index vl j' == ve);
+          assert (I.index itsl j' == to_vlog_entry ve);
+          let i' = i2s_map itsl j' in
+          if fst i' = tid 
+          then (
+            assert (Seq.index thread_log_tid (snd i') == to_vlog_entry ve)
+          );
+          admit()
+        )
+   in
+   assert (SA.prefix thread_log_tid 0 `Seq.equal` empty);
+   assert (SA.prefix vl' 0 `Seq.equal` Seq.empty);
+   lemma_reduce_empty EACInit (trans_fn (seq_machine_of eac_sm));
+   aux 0 0 EACInit (init_thread_state tid)
 
 
 (* when the eac_state of k is instore, then k is in the store of a unique verifier thread *)
